unsymbolized

src/HOL/MicroJava/J/TypeRel.thy
@@ -9,15 +9,15 @@ The relations between Java types
 TypeRel = Decl +
 
 consts
-  subcls1	:: "'c prog \\<Rightarrow> (cname \\<times> cname) set"  (* subclass *)
-  widen 	:: "'c prog \\<Rightarrow> (ty    \\<times> ty   ) set"  (* widening *)
-  cast		:: "'c prog \\<Rightarrow> (cname \\<times> cname) set"  (* casting *)
+  subcls1	:: "'c prog => (cname \\<times> cname) set"  (* subclass *)
+  widen 	:: "'c prog => (ty    \\<times> ty   ) set"  (* widening *)
+  cast		:: "'c prog => (cname \\<times> cname) set"  (* casting *)
 
 syntax
-  subcls1	:: "'c prog \\<Rightarrow> [cname, cname] \\<Rightarrow> bool" ("_\\<turnstile>_\\<prec>C1_"	 [71,71,71] 70)
-  subcls	:: "'c prog \\<Rightarrow> [cname, cname] \\<Rightarrow> bool" ("_\\<turnstile>_\\<preceq>C _"	 [71,71,71] 70)
-  widen		:: "'c prog \\<Rightarrow> [ty   , ty   ] \\<Rightarrow> bool" ("_\\<turnstile>_\\<preceq>_"  [71,71,71] 70)
-  cast		:: "'c prog \\<Rightarrow> [cname, cname] \\<Rightarrow> bool" ("_\\<turnstile>_\\<preceq>? _"[71,71,71] 70)
+  subcls1	:: "'c prog => [cname, cname] => bool" ("_\\<turnstile>_\\<prec>C1_"	 [71,71,71] 70)
+  subcls	:: "'c prog => [cname, cname] => bool" ("_\\<turnstile>_\\<preceq>C _"	 [71,71,71] 70)
+  widen		:: "'c prog => [ty   , ty   ] => bool" ("_\\<turnstile>_\\<preceq>_"  [71,71,71] 70)
+  cast		:: "'c prog => [cname, cname] => bool" ("_\\<turnstile>_\\<preceq>? _"[71,71,71] 70)
 
 translations
   	"G\\<turnstile>C \\<prec>C1 D" == "(C,D) \\<in> subcls1 G"
@@ -28,23 +28,23 @@ translations
 defs
 
   (* direct subclass, cf. 8.1.3 *)
-  subcls1_def	"subcls1 G \\<equiv> {(C,D). \\<exists>c. class G C = Some c \\<and> fst c = Some D}"
+  subcls1_def	"subcls1 G == {(C,D). \\<exists>c. class G C = Some c \\<and> fst c = Some D}"
   
 consts
 
-  method	:: "'c prog \\<times> cname \\<Rightarrow> ( sig   \\<leadsto> cname \\<times> ty \\<times> 'c)"
-  field	:: "'c prog \\<times> cname \\<Rightarrow> ( vname \\<leadsto> cname \\<times> ty)"
-  fields	:: "'c prog \\<times> cname \\<Rightarrow> ((vname \\<times> cname) \\<times>  ty) list"
+  method	:: "'c prog \\<times> cname => ( sig   \\<leadsto> cname \\<times> ty \\<times> 'c)"
+  field	:: "'c prog \\<times> cname => ( vname \\<leadsto> cname \\<times> ty)"
+  fields	:: "'c prog \\<times> cname => ((vname \\<times> cname) \\<times>  ty) list"
 
 constdefs       (* auxiliary relations for recursive definitions below *)
 
   subcls1_rel	:: "(('c prog \\<times> cname) \\<times> ('c prog \\<times> cname)) set"
- "subcls1_rel \\<equiv> {((G,C),(G',C')). G = G' \\<and>  wf ((subcls1 G)^-1) \\<and>  G\\<turnstile>C'\\<prec>C1C}"
+ "subcls1_rel == {((G,C),(G',C')). G = G' \\<and>  wf ((subcls1 G)^-1) \\<and>  G\\<turnstile>C'\\<prec>C1C}"
 
 (* methods of a class, with inheritance, overriding and hiding, cf. 8.4.6 *)
 recdef method "subcls1_rel"
- "method (G,C) = (if wf((subcls1 G)^-1) then (case class G C of None \\<Rightarrow> empty
-                   | Some (sc,fs,ms) \\<Rightarrow> (case sc of None \\<Rightarrow> empty | Some D \\<Rightarrow> 
+ "method (G,C) = (if wf((subcls1 G)^-1) then (case class G C of None => empty
+                   | Some (sc,fs,ms) => (case sc of None => empty | Some D => 
                                            if is_class G D then method (G,D) 
                                                            else arbitrary) \\<oplus>
                                            map_of (map (\\<lambda>(s,  m ). 
@@ -53,25 +53,25 @@ recdef method "subcls1_rel"
 
 (* list of fields of a class, including inherited and hidden ones *)
 recdef fields  "subcls1_rel"
- "fields (G,C) = (if wf((subcls1 G)^-1) then (case class G C of None \\<Rightarrow> arbitrary
-                   | Some (sc,fs,ms) \\<Rightarrow> map (\\<lambda>(fn,ft). ((fn,C),ft)) fs@
-                                           (case sc of None \\<Rightarrow> [] | Some D \\<Rightarrow> 
+ "fields (G,C) = (if wf((subcls1 G)^-1) then (case class G C of None => arbitrary
+                   | Some (sc,fs,ms) => map (\\<lambda>(fn,ft). ((fn,C),ft)) fs@
+                                           (case sc of None => [] | Some D => 
                                            if is_class G D then fields (G,D) 
                                                            else arbitrary))
                   else arbitrary)"
 defs
 
-  field_def "field \\<equiv> map_of o (map (\\<lambda>((fn,fd),ft). (fn,(fd,ft)))) o fields"
+  field_def "field == map_of o (map (\\<lambda>((fn,fd),ft). (fn,(fd,ft)))) o fields"
 
 inductive "widen G" intrs (*widening, viz. method invocation conversion, cf. 5.3
 			     i.e. sort of syntactic subtyping *)
   refl	             "G\\<turnstile>      T \\<preceq> T" 	 (* identity conv., cf. 5.1.1 *)
-  subcls "G\\<turnstile>C\\<preceq>C D \\<Longrightarrow> G\\<turnstile>Class C \\<preceq> Class D"
+  subcls "G\\<turnstile>C\\<preceq>C D ==> G\\<turnstile>Class C \\<preceq> Class D"
   null	             "G\\<turnstile>     NT \\<preceq> RefT R"
 
 inductive "cast G" intrs (* casting conversion, cf. 5.5 / 5.1.5 *)
                          (* left out casts on primitve types    *)
-  widen	 "G\\<turnstile>C\\<preceq>C D \\<Longrightarrow> G\\<turnstile>C \\<preceq>? D"
-  subcls "G\\<turnstile>D\\<preceq>C C \\<Longrightarrow> G\\<turnstile>C \\<preceq>? D"
+  widen	 "G\\<turnstile>C\\<preceq>C D ==> G\\<turnstile>C \\<preceq>? D"
+  subcls "G\\<turnstile>D\\<preceq>C C ==> G\\<turnstile>C \\<preceq>? D"
 
 end
