src/HOL/MicroJava/BV/BVSpec.thy
@@ -11,53 +11,53 @@ theory BVSpec = Step:
 
 types
  method_type = "state_type option list"
- class_type	 = "sig \<Rightarrow> method_type"
- prog_type	 = "cname \<Rightarrow> class_type"
+ class_type	 = "sig => method_type"
+ prog_type	 = "cname => class_type"
 
 constdefs
-wt_instr :: "[instr,jvm_prog,ty,method_type,p_count,p_count] \<Rightarrow> bool"
-"wt_instr i G rT phi max_pc pc \<equiv> 
+wt_instr :: "[instr,jvm_prog,ty,method_type,p_count,p_count] => bool"
+"wt_instr i G rT phi max_pc pc == 
     app i G rT (phi!pc) \<and>
    (\<forall> pc' \<in> set (succs i pc). pc' < max_pc \<and> (G \<turnstile> step i G (phi!pc) <=' phi!pc'))"
 
-wt_start :: "[jvm_prog,cname,ty list,nat,method_type] \<Rightarrow> bool"
-"wt_start G C pTs mxl phi \<equiv> 
+wt_start :: "[jvm_prog,cname,ty list,nat,method_type] => bool"
+"wt_start G C pTs mxl phi == 
     G \<turnstile> Some ([],(Ok (Class C))#((map Ok pTs))@(replicate mxl Err)) <=' phi!0"
 
 
-wt_method :: "[jvm_prog,cname,ty list,ty,nat,instr list,method_type] \<Rightarrow> bool"
-"wt_method G C pTs rT mxl ins phi \<equiv>
+wt_method :: "[jvm_prog,cname,ty list,ty,nat,instr list,method_type] => bool"
+"wt_method G C pTs rT mxl ins phi ==
 	let max_pc = length ins
         in
 	0 < max_pc \<and> wt_start G C pTs mxl phi \<and> 
-	(\<forall>pc. pc<max_pc \<longrightarrow> wt_instr (ins ! pc) G rT phi max_pc pc)"
+	(\<forall>pc. pc<max_pc --> wt_instr (ins ! pc) G rT phi max_pc pc)"
 
-wt_jvm_prog :: "[jvm_prog,prog_type] \<Rightarrow> bool"
-"wt_jvm_prog G phi \<equiv>
+wt_jvm_prog :: "[jvm_prog,prog_type] => bool"
+"wt_jvm_prog G phi ==
    wf_prog (\<lambda>G C (sig,rT,maxl,b).
               wt_method G C (snd sig) rT maxl b (phi C sig)) G"
 
 
 
 lemma wt_jvm_progD:
-"wt_jvm_prog G phi \<Longrightarrow> (\<exists>wt. wf_prog wt G)"
+"wt_jvm_prog G phi ==> (\<exists>wt. wf_prog wt G)"
 by (unfold wt_jvm_prog_def, blast)
 
 lemma wt_jvm_prog_impl_wt_instr:
-"\<lbrakk> wt_jvm_prog G phi; method (G,C) sig = Some (C,rT,maxl,ins); pc < length ins \<rbrakk> 
- \<Longrightarrow> wt_instr (ins!pc) G rT (phi C sig) (length ins) pc";
+"[| wt_jvm_prog G phi; method (G,C) sig = Some (C,rT,maxl,ins); pc < length ins |] 
+ ==> wt_instr (ins!pc) G rT (phi C sig) (length ins) pc";
 by (unfold wt_jvm_prog_def, drule method_wf_mdecl, 
     simp, simp add: wf_mdecl_def wt_method_def)
 
 lemma wt_jvm_prog_impl_wt_start:
-"\<lbrakk> wt_jvm_prog G phi; method (G,C) sig = Some (C,rT,maxl,ins) \<rbrakk> \<Longrightarrow> 
+"[| wt_jvm_prog G phi; method (G,C) sig = Some (C,rT,maxl,ins) |] ==> 
  0 < (length ins) \<and> wt_start G C (snd sig) maxl (phi C sig)"
 by (unfold wt_jvm_prog_def, drule method_wf_mdecl, 
     simp, simp add: wf_mdecl_def wt_method_def)
 
 (* for most instructions wt_instr collapses: *)
 lemma  
-"succs i pc = [pc+1] \<Longrightarrow> wt_instr i G rT phi max_pc pc = 
+"succs i pc = [pc+1] ==> wt_instr i G rT phi max_pc pc = 
  (app i G rT (phi!pc) \<and> pc+1 < max_pc \<and> (G \<turnstile> step i G (phi!pc) <=' phi!(pc+1)))"
 by (simp add: wt_instr_def) 
 
