src/HOL/MicroJava/J/Decl.thy
@@ -32,26 +32,26 @@ consts
 
 defs 
 
- ObjectC_def "ObjectC \\<equiv> (Object, (None, [], []))"
+ ObjectC_def "ObjectC == (Object, (None, [], []))"
 
 
 types 'c prog = "'c cdecl list"
 
 consts
 
-  class		:: "'c prog \\<Rightarrow> (cname \\<leadsto> 'c class)"
+  class		:: "'c prog => (cname \\<leadsto> 'c class)"
 
-  is_class	:: "'c prog \\<Rightarrow> cname \\<Rightarrow> bool"
-  is_type	:: "'c prog \\<Rightarrow> ty    \\<Rightarrow> bool"
+  is_class	:: "'c prog => cname => bool"
+  is_type	:: "'c prog => ty    => bool"
 
 defs
 
-  class_def	"class        \\<equiv> map_of"
+  class_def	"class        == map_of"
 
-  is_class_def	"is_class G C \\<equiv> class G C \\<noteq> None"
+  is_class_def	"is_class G C == class G C \\<noteq> None"
 
 primrec
 "is_type G (PrimT pt) = True"
-"is_type G (RefT t) = (case t of NullT \\<Rightarrow> True | ClassT C \\<Rightarrow> is_class G C)"
+"is_type G (RefT t) = (case t of NullT => True | ClassT C => is_class G C)"
 
 end
