src/HOL/MicroJava/J/Eval.thy
@@ -10,118 +10,118 @@ execution of Java expressions and statements
 Eval = State + WellType +
 
 consts
-  eval  :: "java_mb prog \\<Rightarrow> (xstate \\<times> expr      \\<times> val      \\<times> xstate) set"
-  evals :: "java_mb prog \\<Rightarrow> (xstate \\<times> expr list \\<times> val list \\<times> xstate) set"
-  exec  :: "java_mb prog \\<Rightarrow> (xstate \\<times> stmt                 \\<times> xstate) set"
+  eval  :: "java_mb prog => (xstate \\<times> expr      \\<times> val      \\<times> xstate) set"
+  evals :: "java_mb prog => (xstate \\<times> expr list \\<times> val list \\<times> xstate) set"
+  exec  :: "java_mb prog => (xstate \\<times> stmt                 \\<times> xstate) set"
 
 syntax
-  eval :: "[java_mb prog,xstate,expr,val,xstate] \\<Rightarrow> bool "("_\\<turnstile>_ -_\\<succ>_\\<rightarrow> _"[51,82,82,82,82]81)
+  eval :: "[java_mb prog,xstate,expr,val,xstate] => bool "("_\\<turnstile>_ -_\\<succ>_-> _"[51,82,82,82,82]81)
   evals:: "[java_mb prog,xstate,expr list,
-	                      val list,xstate] \\<Rightarrow> bool "("_\\<turnstile>_ -_[\\<succ>]_\\<rightarrow> _"[51,82,51,51,82]81)
-  exec :: "[java_mb prog,xstate,stmt,    xstate] \\<Rightarrow> bool "("_\\<turnstile>_ -_\\<rightarrow> _"  [51,82,82,   82]81)
+	                      val list,xstate] => bool "("_\\<turnstile>_ -_[\\<succ>]_-> _"[51,82,51,51,82]81)
+  exec :: "[java_mb prog,xstate,stmt,    xstate] => bool "("_\\<turnstile>_ -_-> _"  [51,82,82,   82]81)
 
 translations
-  "G\\<turnstile>s -e \\<succ> v\\<rightarrow> (x,s')" <= "(s, e, v, x, s') \\<in> eval  G"
-  "G\\<turnstile>s -e \\<succ> v\\<rightarrow>    s' " == "(s, e, v,    s' ) \\<in> eval  G"
-  "G\\<turnstile>s -e[\\<succ>]v\\<rightarrow> (x,s')" <= "(s, e, v, x, s') \\<in> evals G"
-  "G\\<turnstile>s -e[\\<succ>]v\\<rightarrow>    s' " == "(s, e, v,    s' ) \\<in> evals G"
-  "G\\<turnstile>s -c    \\<rightarrow> (x,s')" <= "(s, c, x, s') \\<in> exec  G"
-  "G\\<turnstile>s -c    \\<rightarrow>    s' " == "(s, c,    s') \\<in> exec  G"
+  "G\\<turnstile>s -e \\<succ> v-> (x,s')" <= "(s, e, v, x, s') \\<in> eval  G"
+  "G\\<turnstile>s -e \\<succ> v->    s' " == "(s, e, v,    s' ) \\<in> eval  G"
+  "G\\<turnstile>s -e[\\<succ>]v-> (x,s')" <= "(s, e, v, x, s') \\<in> evals G"
+  "G\\<turnstile>s -e[\\<succ>]v->    s' " == "(s, e, v,    s' ) \\<in> evals G"
+  "G\\<turnstile>s -c    -> (x,s')" <= "(s, c, x, s') \\<in> exec  G"
+  "G\\<turnstile>s -c    ->    s' " == "(s, c,    s') \\<in> exec  G"
 
 inductive "eval G" "evals G" "exec G" intrs
 
 (* evaluation of expressions *)
 
   (* cf. 15.5 *)
-  XcptE				  "G\\<turnstile>(Some xc,s) -e\\<succ>arbitrary\\<rightarrow> (Some xc,s)"
+  XcptE				  "G\\<turnstile>(Some xc,s) -e\\<succ>arbitrary-> (Some xc,s)"
 
   (* cf. 15.8.1 *)
-  NewC	"\\<lbrakk>h = heap s; (a,x) = new_Addr h;
-	  h'= h(a\\<mapsto>(C,init_vars (fields (G,C))))\\<rbrakk> \\<Longrightarrow>
-				   G\\<turnstile>Norm s -NewC C\\<succ>Addr a\\<rightarrow> c_hupd h' (x,s)"
+  NewC	"[|h = heap s; (a,x) = new_Addr h;
+	  h'= h(a\\<mapsto>(C,init_vars (fields (G,C))))|] ==>
+				   G\\<turnstile>Norm s -NewC C\\<succ>Addr a-> c_hupd h' (x,s)"
 
   (* cf. 15.15 *)
-  Cast	"\\<lbrakk>G\\<turnstile>Norm s0 -e\\<succ>v\\<rightarrow> (x1,s1);
-	  x2=raise_if (\\<not> cast_ok G C (heap s1) v) ClassCast x1\\<rbrakk> \\<Longrightarrow>
-			        G\\<turnstile>Norm s0 -Cast C e\\<succ>v\\<rightarrow> (x2,s1)"
+  Cast	"[|G\\<turnstile>Norm s0 -e\\<succ>v-> (x1,s1);
+	  x2=raise_if (\\<not> cast_ok G C (heap s1) v) ClassCast x1|] ==>
+			        G\\<turnstile>Norm s0 -Cast C e\\<succ>v-> (x2,s1)"
 
   (* cf. 15.7.1 *)
-  Lit				   "G\\<turnstile>Norm s -Lit v\\<succ>v\\<rightarrow> Norm s"
+  Lit				   "G\\<turnstile>Norm s -Lit v\\<succ>v-> Norm s"
 
-  BinOp "\\<lbrakk>G\\<turnstile>Norm s -e1\\<succ>v1\\<rightarrow> s1;
-	  G\\<turnstile>s1     -e2\\<succ>v2\\<rightarrow> s2;
-	  v = (case bop of Eq  \\<Rightarrow> Bool (v1 = v2)
-	                 | Add \\<Rightarrow> Intg (the_Intg v1 + the_Intg v2))\\<rbrakk> \\<Longrightarrow>
-				   G\\<turnstile>Norm s -BinOp bop e1 e2\\<succ>v\\<rightarrow> s2"
+  BinOp "[|G\\<turnstile>Norm s -e1\\<succ>v1-> s1;
+	  G\\<turnstile>s1     -e2\\<succ>v2-> s2;
+	  v = (case bop of Eq  => Bool (v1 = v2)
+	                 | Add => Intg (the_Intg v1 + the_Intg v2))|] ==>
+				   G\\<turnstile>Norm s -BinOp bop e1 e2\\<succ>v-> s2"
 
   (* cf. 15.13.1, 15.2 *)
-  LAcc				  "G\\<turnstile>Norm s -LAcc v\\<succ>the (locals s v)\\<rightarrow> Norm s"
+  LAcc				  "G\\<turnstile>Norm s -LAcc v\\<succ>the (locals s v)-> Norm s"
 
   (* cf. 15.25.1 *)
-  LAss  "\\<lbrakk>G\\<turnstile>Norm s -e\\<succ>v\\<rightarrow>  (x,(h,l));
-	  l' = (if x = None then l(va\\<mapsto>v) else l)\\<rbrakk> \\<Longrightarrow>
-				   G\\<turnstile>Norm s -va\\<Colon>=e\\<succ>v\\<rightarrow> (x,(h,l'))"
+  LAss  "[|G\\<turnstile>Norm s -e\\<succ>v->  (x,(h,l));
+	  l' = (if x = None then l(va\\<mapsto>v) else l)|] ==>
+				   G\\<turnstile>Norm s -va::=e\\<succ>v-> (x,(h,l'))"
 
 
   (* cf. 15.10.1, 15.2 *)
-  FAcc	"\\<lbrakk>G\\<turnstile>Norm s0 -e\\<succ>a'\\<rightarrow> (x1,s1); 
-	  v = the (snd (the (heap s1 (the_Addr a'))) (fn,T))\\<rbrakk> \\<Longrightarrow>
-				 G\\<turnstile>Norm s0 -{T}e..fn\\<succ>v\\<rightarrow> (np a' x1,s1)"
+  FAcc	"[|G\\<turnstile>Norm s0 -e\\<succ>a'-> (x1,s1); 
+	  v = the (snd (the (heap s1 (the_Addr a'))) (fn,T))|] ==>
+				 G\\<turnstile>Norm s0 -{T}e..fn\\<succ>v-> (np a' x1,s1)"
 
   (* cf. 15.25.1 *)
-  FAss  "\\<lbrakk>G\\<turnstile>     Norm s0  -e1\\<succ>a'\\<rightarrow> (x1,s1); a = the_Addr a';
-	  G\\<turnstile>(np a' x1,s1) -e2\\<succ>v \\<rightarrow> (x2,s2);
+  FAss  "[|G\\<turnstile>     Norm s0  -e1\\<succ>a'-> (x1,s1); a = the_Addr a';
+	  G\\<turnstile>(np a' x1,s1) -e2\\<succ>v -> (x2,s2);
 	  h = heap s2; (c,fs) = the (h a);
-	  h' = h(a\\<mapsto>(c,(fs((fn,T)\\<mapsto>v))))\\<rbrakk> \\<Longrightarrow>
-			  G\\<turnstile>Norm s0 -{T}e1..fn:=e2\\<succ>v\\<rightarrow> c_hupd h' (x2,s2)"
+	  h' = h(a\\<mapsto>(c,(fs((fn,T)\\<mapsto>v))))|] ==>
+			  G\\<turnstile>Norm s0 -{T}e1..fn:=e2\\<succ>v-> c_hupd h' (x2,s2)"
 
   (* cf. 15.11.4.1, 15.11.4.2, 15.11.4.4, 15.11.4.5, 14.15 *)
-  Call	"\\<lbrakk>G\\<turnstile>Norm s0 -e\\<succ>a'\\<rightarrow> s1; a = the_Addr a';
-	   G\\<turnstile>s1 -ps[\\<succ>]pvs\\<rightarrow> (x,(h,l)); dynT = fst (the (h a));
+  Call	"[|G\\<turnstile>Norm s0 -e\\<succ>a'-> s1; a = the_Addr a';
+	   G\\<turnstile>s1 -ps[\\<succ>]pvs-> (x,(h,l)); dynT = fst (the (h a));
 	   (md,rT,pns,lvars,blk,res) = the (method (G,dynT) (mn,pTs));
-	   G\\<turnstile>(np a' x,(h,(init_vars lvars)(pns[\\<mapsto>]pvs)(This\\<mapsto>a'))) -blk\\<rightarrow> s3;
-	   G\\<turnstile>     s3 -res\\<succ>v \\<rightarrow> (x4,s4)\\<rbrakk> \\<Longrightarrow>
-			    G\\<turnstile>Norm s0 -e..mn({pTs}ps)\\<succ>v\\<rightarrow> (x4,(heap s4,l))"
+	   G\\<turnstile>(np a' x,(h,(init_vars lvars)(pns[\\<mapsto>]pvs)(This\\<mapsto>a'))) -blk-> s3;
+	   G\\<turnstile>     s3 -res\\<succ>v -> (x4,s4)|] ==>
+			    G\\<turnstile>Norm s0 -e..mn({pTs}ps)\\<succ>v-> (x4,(heap s4,l))"
 
 
 (* evaluation of expression lists *)
 
   (* cf. 15.5 *)
-  XcptEs			  "G\\<turnstile>(Some xc,s) -e[\\<succ>]arbitrary\\<rightarrow> (Some xc,s)"
+  XcptEs			  "G\\<turnstile>(Some xc,s) -e[\\<succ>]arbitrary-> (Some xc,s)"
 
   (* cf. 15.11.??? *)
   Nil
-				    "G\\<turnstile>Norm s0 -[][\\<succ>][]\\<rightarrow> Norm s0"
+				    "G\\<turnstile>Norm s0 -[][\\<succ>][]-> Norm s0"
 
   (* cf. 15.6.4 *)
-  Cons	"\\<lbrakk>G\\<turnstile>Norm s0 -e  \\<succ> v \\<rightarrow> s1;
-           G\\<turnstile>     s1 -es[\\<succ>]vs\\<rightarrow> s2\\<rbrakk> \\<Longrightarrow>
-				   G\\<turnstile>Norm s0 -e#es[\\<succ>]v#vs\\<rightarrow> s2"
+  Cons	"[|G\\<turnstile>Norm s0 -e  \\<succ> v -> s1;
+           G\\<turnstile>     s1 -es[\\<succ>]vs-> s2|] ==>
+				   G\\<turnstile>Norm s0 -e#es[\\<succ>]v#vs-> s2"
 
 (* execution of statements *)
 
   (* cf. 14.1 *)
-  XcptS				 "G\\<turnstile>(Some xc,s) -s0\\<rightarrow> (Some xc,s)"
+  XcptS				 "G\\<turnstile>(Some xc,s) -s0-> (Some xc,s)"
 
   (* cf. 14.5 *)
-  Skip	 			    "G\\<turnstile>Norm s -Skip\\<rightarrow> Norm s"
+  Skip	 			    "G\\<turnstile>Norm s -Skip-> Norm s"
 
   (* cf. 14.7 *)
-  Expr	"\\<lbrakk>G\\<turnstile>Norm s0 -e\\<succ>v\\<rightarrow> s1\\<rbrakk> \\<Longrightarrow>
-				  G\\<turnstile>Norm s0 -Expr e\\<rightarrow> s1"
+  Expr	"[|G\\<turnstile>Norm s0 -e\\<succ>v-> s1|] ==>
+				  G\\<turnstile>Norm s0 -Expr e-> s1"
 
   (* cf. 14.2 *)
-  Comp	"\\<lbrakk>G\\<turnstile>Norm s0 -s \\<rightarrow> s1;
-	  G\\<turnstile>     s1 -t \\<rightarrow> s2\\<rbrakk> \\<Longrightarrow>
-				 G\\<turnstile>Norm s0 -(s;; t)\\<rightarrow> s2"
+  Comp	"[|G\\<turnstile>Norm s0 -s -> s1;
+	  G\\<turnstile>     s1 -t -> s2|] ==>
+				 G\\<turnstile>Norm s0 -(s;; t)-> s2"
 
   (* cf. 14.8.2 *)
-  Cond	"\\<lbrakk>G\\<turnstile>Norm s0  -e \\<succ>v\\<rightarrow> s1;
-	  G\\<turnstile>     s1 -(if  the_Bool v then s else t)\\<rightarrow> s2\\<rbrakk> \\<Longrightarrow>
-		        G\\<turnstile>Norm s0 -(If(e) s Else t)\\<rightarrow> s2"
+  Cond	"[|G\\<turnstile>Norm s0  -e \\<succ>v-> s1;
+	  G\\<turnstile>     s1 -(if  the_Bool v then s else t)-> s2|] ==>
+		        G\\<turnstile>Norm s0 -(If(e) s Else t)-> s2"
 
   (* cf. 14.10, 14.10.1 *)
-  Loop	"\\<lbrakk>G\\<turnstile>Norm s0 -(If(e) (s;; While(e) s) Else Skip)\\<rightarrow> s1\\<rbrakk> \\<Longrightarrow>
-			    G\\<turnstile>Norm s0 -(While(e) s)\\<rightarrow> s1"
+  Loop	"[|G\\<turnstile>Norm s0 -(If(e) (s;; While(e) s) Else Skip)-> s1|] ==>
+			    G\\<turnstile>Norm s0 -(While(e) s)-> s1"
 
 end
