src/HOL/MicroJava/J/Term.thy
@@ -16,7 +16,7 @@ datatype expr
 	| Lit	val		   (* literal value, also references *)
         | BinOp binop  expr expr   (* binary operation *)
 	| LAcc vname		   (* local (incl. parameter) access *)
-	| LAss vname expr          (* local assign *) ("_\\<Colon>=_"  [      90,90]90)
+	| LAss vname expr          (* local assign *) ("_::=_"  [      90,90]90)
 	| FAcc cname expr vname    (* field access *) ("{_}_.._"[10,90,99   ]90)
 	| FAss cname expr vname 
 	                  expr     (* field ass. *)("{_}_.._:=_"[10,90,99,90]90)
