src/HOL/MicroJava/J/WellForm.thy
@@ -20,28 +20,28 @@ types 'c wf_mb = 'c prog => cname => 'c mdecl => bool
 
 constdefs
 
- wf_fdecl	:: "'c prog \\<Rightarrow>          fdecl \\<Rightarrow> bool"
-"wf_fdecl G \\<equiv> \\<lambda>(fn,ft). is_type G ft"
+ wf_fdecl	:: "'c prog =>          fdecl => bool"
+"wf_fdecl G == \\<lambda>(fn,ft). is_type G ft"
 
- wf_mhead	:: "'c prog \\<Rightarrow> sig   \\<Rightarrow> ty \\<Rightarrow> bool"
-"wf_mhead G \\<equiv> \\<lambda>(mn,pTs) rT. (\\<forall>T\\<in>set pTs. is_type G T) \\<and> is_type G rT"
+ wf_mhead	:: "'c prog => sig   => ty => bool"
+"wf_mhead G == \\<lambda>(mn,pTs) rT. (\\<forall>T\\<in>set pTs. is_type G T) \\<and> is_type G rT"
 
- wf_mdecl	:: "'c wf_mb \\<Rightarrow> 'c wf_mb"
-"wf_mdecl wf_mb G C \\<equiv> \\<lambda>(sig,rT,mb). wf_mhead G sig rT \\<and> wf_mb G C (sig,rT,mb)"
+ wf_mdecl	:: "'c wf_mb => 'c wf_mb"
+"wf_mdecl wf_mb G C == \\<lambda>(sig,rT,mb). wf_mhead G sig rT \\<and> wf_mb G C (sig,rT,mb)"
 
-  wf_cdecl	:: "'c wf_mb \\<Rightarrow> 'c prog \\<Rightarrow> 'c cdecl \\<Rightarrow> bool"
-"wf_cdecl wf_mb G \\<equiv>
+  wf_cdecl	:: "'c wf_mb => 'c prog => 'c cdecl => bool"
+"wf_cdecl wf_mb G ==
    \\<lambda>(C,(sc,fs,ms)).
 	(\\<forall>f\\<in>set fs. wf_fdecl G   f    ) \\<and>  unique fs \\<and>
 	(\\<forall>m\\<in>set ms. wf_mdecl wf_mb G C m) \\<and>  unique ms \\<and>
-	(case sc of None \\<Rightarrow> C = Object
-         | Some D \\<Rightarrow>
+	(case sc of None => C = Object
+         | Some D =>
              is_class G D \\<and>  \\<not>  G\\<turnstile>D\\<preceq>C C \\<and>
              (\\<forall>(sig,rT,b)\\<in>set ms. \\<forall>D' rT' b'.
-                 method(G,D) sig = Some(D',rT',b') \\<longrightarrow> G\\<turnstile>rT\\<preceq>rT'))"
+                 method(G,D) sig = Some(D',rT',b') --> G\\<turnstile>rT\\<preceq>rT'))"
 
- wf_prog	:: "'c wf_mb \\<Rightarrow> 'c prog \\<Rightarrow> bool"
-"wf_prog wf_mb G \\<equiv>
+ wf_prog	:: "'c wf_mb => 'c prog => bool"
+"wf_prog wf_mb G ==
    let cs = set G in ObjectC \\<in> cs \\<and> (\\<forall>c\\<in>cs. wf_cdecl wf_mb G c) \\<and> unique G"
 
 end
