src/HOL/MicroJava/J/WellType.thy
@@ -24,8 +24,8 @@ types	lenv (* local variables, including method parameters and This *)
 
 syntax
 
-  prg		:: "'c env \\<Rightarrow> 'c prog"
-  localT	:: "'c env \\<Rightarrow> (vname \\<leadsto> ty)"
+  prg		:: "'c env => 'c prog"
+  localT	:: "'c env => (vname \\<leadsto> ty)"
 
 translations	
 
@@ -34,29 +34,29 @@ translations
 
 consts
 
-  more_spec	:: "'c prog \\<Rightarrow> (ty \\<times> 'x) \\<times> ty list \\<Rightarrow>
-		               (ty \\<times> 'x) \\<times> ty list \\<Rightarrow> bool"
-  appl_methds	:: "'c prog \\<Rightarrow>  cname \\<Rightarrow> sig \\<Rightarrow> ((ty \\<times> ty) \\<times> ty list) set"
-  max_spec	:: "'c prog \\<Rightarrow>  cname \\<Rightarrow> sig \\<Rightarrow> ((ty \\<times> ty) \\<times> ty list) set"
+  more_spec	:: "'c prog => (ty \\<times> 'x) \\<times> ty list =>
+		               (ty \\<times> 'x) \\<times> ty list => bool"
+  appl_methds	:: "'c prog =>  cname => sig => ((ty \\<times> ty) \\<times> ty list) set"
+  max_spec	:: "'c prog =>  cname => sig => ((ty \\<times> ty) \\<times> ty list) set"
 
 defs
 
-  more_spec_def	  "more_spec G \\<equiv> \\<lambda>((d,h),pTs). \\<lambda>((d',h'),pTs'). G\\<turnstile>d\\<preceq>d' \\<and>
+  more_spec_def	  "more_spec G == \\<lambda>((d,h),pTs). \\<lambda>((d',h'),pTs'). G\\<turnstile>d\\<preceq>d' \\<and>
 		                  list_all2 (\\<lambda>T T'. G\\<turnstile>T\\<preceq>T') pTs pTs'"
   
   (* applicable methods, cf. 15.11.2.1 *)
-  appl_methds_def "appl_methds G C \\<equiv> \\<lambda>(mn, pTs).
+  appl_methds_def "appl_methds G C == \\<lambda>(mn, pTs).
 		                 {((Class md,rT),pTs') |md rT mb pTs'.
 		                  method (G,C)  (mn, pTs') = Some (md,rT,mb) \\<and>
 		                  list_all2 (\\<lambda>T T'. G\\<turnstile>T\\<preceq>T') pTs pTs'}"
 
   (* maximally specific methods, cf. 15.11.2.2 *)
-   max_spec_def	  "max_spec G C sig \\<equiv> {m. m \\<in>appl_methds G C sig \\<and> 
+   max_spec_def	  "max_spec G C sig == {m. m \\<in>appl_methds G C sig \\<and> 
 				          (\\<forall>m'\\<in>appl_methds G C sig.
-				                   more_spec G m' m \\<longrightarrow> m' = m)}"
+				                   more_spec G m' m --> m' = m)}"
 consts
 
-  typeof :: "(loc \\<Rightarrow> ty option) \\<Rightarrow> val \\<Rightarrow> ty option"
+  typeof :: "(loc => ty option) => val => ty option"
 
 primrec
 	"typeof dt  Unit    = Some (PrimT Void)"
@@ -71,19 +71,19 @@ types
 
 consts
 
-  ty_expr :: "java_mb env \\<Rightarrow> (expr      \\<times> ty     ) set"
-  ty_exprs:: "java_mb env \\<Rightarrow> (expr list \\<times> ty list) set"
-  wt_stmt :: "java_mb env \\<Rightarrow>  stmt                 set"
+  ty_expr :: "java_mb env => (expr      \\<times> ty     ) set"
+  ty_exprs:: "java_mb env => (expr list \\<times> ty list) set"
+  wt_stmt :: "java_mb env =>  stmt                 set"
 
 syntax
 
-ty_expr :: "java_mb env \\<Rightarrow> [expr     , ty     ] \\<Rightarrow> bool" ("_\\<turnstile>_\\<Colon>_"  [51,51,51]50)
-ty_exprs:: "java_mb env \\<Rightarrow> [expr list, ty list] \\<Rightarrow> bool" ("_\\<turnstile>_[\\<Colon>]_"[51,51,51]50)
-wt_stmt :: "java_mb env \\<Rightarrow>  stmt                \\<Rightarrow> bool" ("_\\<turnstile>_ \\<surd>" [51,51   ]50)
+ty_expr :: "java_mb env => [expr     , ty     ] => bool" ("_\\<turnstile>_::_"  [51,51,51]50)
+ty_exprs:: "java_mb env => [expr list, ty list] => bool" ("_\\<turnstile>_[::]_"[51,51,51]50)
+wt_stmt :: "java_mb env =>  stmt                => bool" ("_\\<turnstile>_ \\<surd>" [51,51   ]50)
 
 translations
-	"E\\<turnstile>e \\<Colon> T" == "(e,T) \\<in> ty_expr  E"
-	"E\\<turnstile>e[\\<Colon>]T" == "(e,T) \\<in> ty_exprs E"
+	"E\\<turnstile>e :: T" == "(e,T) \\<in> ty_expr  E"
+	"E\\<turnstile>e[::]T" == "(e,T) \\<in> ty_exprs E"
 	"E\\<turnstile>c \\<surd>"    == "c     \\<in> wt_stmt  E"
   
 inductive "ty_expr E" "ty_exprs E" "wt_stmt E" intrs
@@ -91,98 +91,98 @@ inductive "ty_expr E" "ty_exprs E" "wt_stmt E" intrs
 (* well-typed expressions *)
 
   (* cf. 15.8 *)
-  NewC	"\\<lbrakk>is_class (prg E) C\\<rbrakk> \\<Longrightarrow>
-						 E\\<turnstile>NewC C\\<Colon>Class C"
+  NewC	"[|is_class (prg E) C|] ==>
+						 E\\<turnstile>NewC C::Class C"
 
   (* cf. 15.15 *)
-  Cast	"\\<lbrakk>E\\<turnstile>e\\<Colon>Class C;
-	  prg E\\<turnstile>C\\<preceq>? D\\<rbrakk> \\<Longrightarrow>
-						 E\\<turnstile>Cast D e\\<Colon>Class D"
+  Cast	"[|E\\<turnstile>e::Class C;
+	  prg E\\<turnstile>C\\<preceq>? D|] ==>
+						 E\\<turnstile>Cast D e::Class D"
 
   (* cf. 15.7.1 *)
-  Lit	"\\<lbrakk>typeof (\\<lambda>v. None) x = Some T\\<rbrakk> \\<Longrightarrow>
-						 E\\<turnstile>Lit x\\<Colon>T"
+  Lit	"[|typeof (\\<lambda>v. None) x = Some T|] ==>
+						 E\\<turnstile>Lit x::T"
 
   
   (* cf. 15.13.1 *)
-  LAcc	"\\<lbrakk>localT E v = Some T; is_type (prg E) T\\<rbrakk> \\<Longrightarrow>
-						 E\\<turnstile>LAcc v\\<Colon>T"
+  LAcc	"[|localT E v = Some T; is_type (prg E) T|] ==>
+						 E\\<turnstile>LAcc v::T"
 
-  BinOp "\\<lbrakk>E\\<turnstile>e1\\<Colon>T;
-	  E\\<turnstile>e2\\<Colon>T;
+  BinOp "[|E\\<turnstile>e1::T;
+	  E\\<turnstile>e2::T;
 	  if bop = Eq then T' = PrimT Boolean
-	              else T' = T \\<and> T = PrimT Integer\\<rbrakk> \\<Longrightarrow>
-						 E\\<turnstile>BinOp bop e1 e2\\<Colon>T'"
+	              else T' = T \\<and> T = PrimT Integer|] ==>
+						 E\\<turnstile>BinOp bop e1 e2::T'"
 
   (* cf. 15.25, 15.25.1 *)
-  LAss  "\\<lbrakk>E\\<turnstile>LAcc v\\<Colon>T;
-	  E\\<turnstile>e\\<Colon>T';
-	  prg E\\<turnstile>T'\\<preceq>T\\<rbrakk> \\<Longrightarrow>
-						 E\\<turnstile>v\\<Colon>=e\\<Colon>T'"
+  LAss  "[|E\\<turnstile>LAcc v::T;
+	  E\\<turnstile>e::T';
+	  prg E\\<turnstile>T'\\<preceq>T|] ==>
+						 E\\<turnstile>v::=e::T'"
 
   (* cf. 15.10.1 *)
-  FAcc	"\\<lbrakk>E\\<turnstile>a\\<Colon>Class C; 
-	  field (prg E,C) fn = Some (fd,fT)\\<rbrakk> \\<Longrightarrow>
-						 E\\<turnstile>{fd}a..fn\\<Colon>fT"
+  FAcc	"[|E\\<turnstile>a::Class C; 
+	  field (prg E,C) fn = Some (fd,fT)|] ==>
+						 E\\<turnstile>{fd}a..fn::fT"
 
   (* cf. 15.25, 15.25.1 *)
-  FAss  "\\<lbrakk>E\\<turnstile>{fd}a..fn\\<Colon>T;
-	  E\\<turnstile>v       \\<Colon>T';
-	  prg E\\<turnstile>T'\\<preceq>T\\<rbrakk> \\<Longrightarrow>
-					 	 E\\<turnstile>{fd}a..fn:=v\\<Colon>T'"
+  FAss  "[|E\\<turnstile>{fd}a..fn::T;
+	  E\\<turnstile>v       ::T';
+	  prg E\\<turnstile>T'\\<preceq>T|] ==>
+					 	 E\\<turnstile>{fd}a..fn:=v::T'"
 
 
   (* cf. 15.11.1, 15.11.2, 15.11.3 *)
-  Call	"\\<lbrakk>E\\<turnstile>a\\<Colon>Class C;
-	  E\\<turnstile>ps[\\<Colon>]pTs;
-	  max_spec (prg E) C (mn, pTs) = {((md,rT),pTs')}\\<rbrakk> \\<Longrightarrow>
-						 E\\<turnstile>a..mn({pTs'}ps)\\<Colon>rT"
+  Call	"[|E\\<turnstile>a::Class C;
+	  E\\<turnstile>ps[::]pTs;
+	  max_spec (prg E) C (mn, pTs) = {((md,rT),pTs')}|] ==>
+						 E\\<turnstile>a..mn({pTs'}ps)::rT"
 
 (* well-typed expression lists *)
 
   (* cf. 15.11.??? *)
-  Nil						"E\\<turnstile>[][\\<Colon>][]"
+  Nil						"E\\<turnstile>[][::][]"
 
   (* cf. 15.11.??? *)
-  Cons	"\\<lbrakk>E\\<turnstile>e\\<Colon>T;
-	   E\\<turnstile>es[\\<Colon>]Ts\\<rbrakk> \\<Longrightarrow>
-						 E\\<turnstile>e#es[\\<Colon>]T#Ts"
+  Cons	"[|E\\<turnstile>e::T;
+	   E\\<turnstile>es[::]Ts|] ==>
+						 E\\<turnstile>e#es[::]T#Ts"
 
 (* well-typed statements *)
 
   Skip					"E\\<turnstile>Skip\\<surd>"
 
-  Expr	"\\<lbrakk>E\\<turnstile>e\\<Colon>T\\<rbrakk> \\<Longrightarrow>
+  Expr	"[|E\\<turnstile>e::T|] ==>
 					 E\\<turnstile>Expr e\\<surd>"
 
-  Comp	"\\<lbrakk>E\\<turnstile>s1\\<surd>; 
-	  E\\<turnstile>s2\\<surd>\\<rbrakk> \\<Longrightarrow>
+  Comp	"[|E\\<turnstile>s1\\<surd>; 
+	  E\\<turnstile>s2\\<surd>|] ==>
 					 E\\<turnstile>s1;; s2\\<surd>"
 
   (* cf. 14.8 *)
-  Cond	"\\<lbrakk>E\\<turnstile>e\\<Colon>PrimT Boolean;
+  Cond	"[|E\\<turnstile>e::PrimT Boolean;
 	  E\\<turnstile>s1\\<surd>;
-	  E\\<turnstile>s2\\<surd>\\<rbrakk> \\<Longrightarrow>
+	  E\\<turnstile>s2\\<surd>|] ==>
 					 E\\<turnstile>If(e) s1 Else s2\\<surd>"
 
   (* cf. 14.10 *)
-  Loop "\\<lbrakk>E\\<turnstile>e\\<Colon>PrimT Boolean;
-	 E\\<turnstile>s\\<surd>\\<rbrakk> \\<Longrightarrow>
+  Loop "[|E\\<turnstile>e::PrimT Boolean;
+	 E\\<turnstile>s\\<surd>|] ==>
 					 E\\<turnstile>While(e) s\\<surd>"
 
 constdefs
 
  wf_java_mdecl :: java_mb prog => cname => java_mb mdecl => bool
-"wf_java_mdecl G C \\<equiv> \\<lambda>((mn,pTs),rT,(pns,lvars,blk,res)).
+"wf_java_mdecl G C == \\<lambda>((mn,pTs),rT,(pns,lvars,blk,res)).
 	length pTs = length pns \\<and>
 	nodups pns \\<and>
 	unique lvars \\<and>
 	(\\<forall>pn\\<in>set pns. map_of lvars pn = None) \\<and>
 	(\\<forall>(vn,T)\\<in>set lvars. is_type G T) &
 	(let E = (G,map_of lvars(pns[\\<mapsto>]pTs)(This\\<mapsto>Class C)) in
-	 E\\<turnstile>blk\\<surd> \\<and> (\\<exists>T. E\\<turnstile>res\\<Colon>T \\<and> G\\<turnstile>T\\<preceq>rT))"
+	 E\\<turnstile>blk\\<surd> \\<and> (\\<exists>T. E\\<turnstile>res::T \\<and> G\\<turnstile>T\\<preceq>rT))"
 
  wf_java_prog :: java_mb prog => bool
-"wf_java_prog G \\<equiv> wf_prog wf_java_mdecl G"
+"wf_java_prog G == wf_prog wf_java_mdecl G"
 
 end
